MultiScalarMul_Abstract_Soundness.ec
@@ -5,28 +5,20 @@ require import BitEncoding StdBigop Bigalg.
 (*---*) import Ring.IntID IntOrder BS2Int.
 (*---*) import Bigint BIA.
 
-require import MultiScalarMul_Abstract.
+require import MultiScalarMul_Abstract MultiScalarMul_Abstract_Setup.
 require import IterationProps.
 
 section.
 
 declare module O <: OutCalls.
-declare module O_Partial <: OutCalls.
-
-declare axiom tableP parg varg : hoare [ O.getT : arg = (parg,varg)
-   ==> res = (fun (j i : int) => (i *** (parg j)) +++ - varg)  ].
-
-declare axiom tablePT parg varg : hoare [ O.getPT : arg = (parg,varg)
-   ==> res.`1 => (res.`2 = (fun (j i : int) =>  (i *** (parg j)) +++ - varg)  /\ (forall i j, res.`2 i j <> idR) )   ].
  
-declare axiom getT_lossless : islossless O.getT.
-
-declare axiom tableP_ph parg varg : phoare [ O.getT : arg = (parg,varg)
-   ==> res = (fun (j i : int) =>  (i *** (parg j)) +++ - varg)  ] = 1%r.
-
 declare axiom tablePT_ph parg varg : phoare [ O.getPT : arg = (parg,varg)
    ==> res.`1 => (res.`2 = (fun (j i : int) =>  (i *** (parg j)) +++ - varg)  /\ (forall i j, res.`2 i j <> idR) )   ] = 1%r.
 
+
+lemma tablePT parg varg : hoare [ O.getPT : arg = (parg,varg)
+   ==> res.`1 => (res.`2 = (fun (j i : int) =>  (i *** (parg j)) +++ - varg)  /\ (forall i j, res.`2 i j <> idR) )   ].
+proof. conseq (tablePT_ph parg varg). auto. qed.
    
 
 lemma helpereqs argacc argtable argic args  : 
@@ -47,127 +39,9 @@ rewrite same_res.
 wp. skip. progress. 
 qed.
 
-lemma multiscalarR_spec argP args argU : 
- hoare [ MultiScalarMul(O).multiScalarMulR : 
-  arg = (argP, args, argU) 
-     ==>  res = (multiScalarMulR  args argP)  ].
-proc. wp.
-while (0 <= ic
- /\ (2 ^ w - 1) *** U = v
- /\ table = (fun (j i : int) =>  (i *** (P j)) +++ - v)
- /\ ic <= T
- /\ acc = ((iteri ic
-            (fun i acc1 => acc1 +++
-              (iteri l
-                 (fun j acc2 => acc2 +++ (2 ^ (w * (ic - 1 - i)) * s j i) *** (P j)) idR)
-                 ) idR)) +++ l *** U).
-wp.
-ecall (helper_specR acc table ic s). simplify.
-wp.
-ecall (doublewtimes_spec acc w). skip. progress. smt(w_pos).
-smt(). smt().
-   rewrite mul_plus_distr.
-rewrite iteriZ.           smt().
-simplify.
-have -> : iteri ic{hr}
-  (fun (i : int) (acc0 : R) =>
-     acc0 +++
-     2 ^ w ***
-     iteri l
-       (fun (j : int) (acc2 : R) =>
-          acc2 +++ 2 ^ (w * (ic{hr} - 1 - i)) * s{hr} j i *** P{hr} j) idR)
-  idR
-     = iteri ic{hr}
-  (fun (i : int) (acc0 : R) =>
-     acc0 +++
-     iteri l
-       (fun (j : int) (acc2 : R) =>
-          acc2 +++ 2 ^ (w * (ic{hr}  - i )) * s{hr} j i *** P{hr} j) idR)
-  idR.
-apply eq_iteri.
-progress.
-rewrite iteriZ. smt(l_pos). congr.
-     apply eq_iteri. move => j acc.
-     progress. congr.
-      have ->: 2 ^ w *** (2 ^ (w * (ic{hr} - 1 - i)) * s{hr} j i *** P{hr} j)
-                = 2 ^ w * 2 ^ (w * (ic{hr} - 1 - i)) * s{hr} j i *** P{hr} j .
-  rewrite mulsc. smt. smt().
-        rewrite - exprD_nneg. smt(w_pos). smt(w_pos). smt().
-pose v := (2 ^ w - 1) *** U{hr}.
-have -> : iteri l
-  (fun (j : int) (acc0 : R) => acc0 +++ (s{hr} j ic{hr} *** P{hr} j +++ -v))
-  idR = iteri l
-  (fun (j : int) (acc0 : R) => acc0 +++ (s{hr} j ic{hr} *** P{hr} j)) idR +++
-     iteri l (fun (j : int) (acc0 : R) => acc0 +++ -v) idR.
-rewrite - iteriZZ. simplify.
-smt(l_pos). apply eq_iteri.  progress. smt.
-simplify.
-rewrite  iteriZZZ.
-simplify. smt(l_pos).
-rewrite kik .
-have ->: (2 ^ w *** (l *** U{hr}) +++ l *** -v) = l *** U{hr}.
-    rewrite /v.
-  rewrite  mulsc. smt.
-  have -> : l *** - (2 ^ w - 1) *** U{hr}
-    = (l * - (2 ^ w - 1)) *** U{hr}. rewrite  nmul_mul.  rewrite neg_mul. auto.
-   rewrite - nplus_dist. congr. smt().
-rewrite iteriS.
-smt(). simplify.
-have ->: 2 ^ 0 = 1. smt(@Int).
-smt().
-wp.
-ecall (tableP P v). wp. skip. progress. smt(T_pos).
-rewrite iteri0. auto. smt.
-rewrite /multiScalarMulInt.
-have -> : ic0 = T. smt().
-simplify.
-  have ->: iteri T
-  (fun (i : int) (acc1 : R) =>
-     acc1 +++
-     iteri l
-       (fun (j : int) (acc2 : R) =>
-          acc2 +++ 2 ^ (w * (T - 1 - i)) * s{hr} j i *** P{hr} j) idR) idR +++
-l *** U{hr} +++ - l *** U{hr}
-       = iteri T
-  (fun (i : int) (acc1 : R) =>
-     acc1 +++
-     iteri l
-       (fun (j : int) (acc2 : R) =>
-          acc2 +++ 2 ^ (w * (T - 1 - i)) * s{hr} j i *** P{hr} j) idR) idR +++
-  (l *** U{hr} +++ - l *** U{hr} ).
-smt(op_assoc).
-rewrite op_inv.
-  rewrite op_id.
-  rewrite /multiScalarMulR.
-auto.
-qed.
-
-
-lemma multiscalarR_spec_ph argP args argU : 
- phoare [ MultiScalarMul(O).multiScalarMulR : 
-  arg = (argP, args, argU) 
-     ==>  res = (multiScalarMulR  args argP)  ] = 1%r.
-phoare split ! 1%r 0%r. auto.
-   proc. wp.
-while true (T - ic). progress.
-wp.
-exists* acc, table, ic, s.
-elim*. move => accV tableV icV sV.
-call helper_specR_total.   
-call (_: arg = (accV, MultiScalarMul_Abstract.w) ==> true).
-proc*. call (doublewtimes_spec_ph accV MultiScalarMul_Abstract.w).
-skip. progress. smt(w_pos). skip.
-progress.
-smt().
-wp. call (_:true). apply getT_lossless. 
-wp. skip. progress. smt().
-hoare. simplify.   
-apply multiscalarR_spec.
-qed.
-
 
 lemma multieqs argP args argU  :
- equiv [ MultiScalarMul(O).multiScalarMulR 
+ equiv [ SimpleComp.multiScalarMulR 
         ~ MultiScalarMul(O).multiScalarMulI :
   arg{2} = (argP, args, argU) /\ ={P,s,U} /\ ={glob O}
      ==>  res{2}.`1 => (res{1} = res{2}.`2)].
@@ -200,7 +74,7 @@ wp.
 smt(). smt(). smt(). smt(). smt(). smt().
    smt(). smt().  smt(). smt(). smt().
 wp. 
-ecall {1} (tableP_ph P{1} v{1} ).
+(* ecall {1} (tableP_ph P{1} v{1} ). *)
 ecall {2} (tablePT_ph P{2} v{2}).    
 wp. skip. progress. smt(). smt().
 have -> :     acc_L = acc_R. smt(). auto.
@@ -214,20 +88,22 @@ lemma multiscalarI_spec_ph argP args  argU :
 proof.
 bypr.
 progress.
-have ih: 1%r = Pr[MultiScalarMul(O).multiScalarMulR(P{m}, s{m}, U{m}) @ &m 
+have ih: 1%r = Pr[SimpleComp.multiScalarMulR(P{m}, s{m}, U{m}) @ &m 
   : res = multiScalarMulR args argP].
 byphoare (_: arg = (argP, args, argU) ==> _).
 conseq (multiscalarR_spec_ph argP args argU). smt(). auto.
 have : Pr[MultiScalarMul(O).multiScalarMulI(P{m}, s{m}, U{m}) @ &m :
    res.`1 => res.`2 = multiScalarMulR args argP] >=
-Pr[MultiScalarMul(O).multiScalarMulR(P{m}, s{m}, U{m}) @ &m :
+Pr[SimpleComp.multiScalarMulR(P{m}, s{m}, U{m}) @ &m :
    res = multiScalarMulR args argP].
-byequiv (_: _ ==> res{2}.`1 => res{2}.`2 = res{1} ).
+byequiv (_: ={glob O} /\ arg{2} = (P{m}, s{m}, U{m}) /\ arg{1} = (P{m}, s{m}, U{m}) ==> res{2}.`1 => res{2}.`2 = res{1} ).
 proc*.
 ecall (multieqs argP args argU).
-skip. progress. smt(). smt(). smt(). smt().
+skip. progress. smt(). smt(). smt(). 
 auto.
 smt().
+smt.
+auto.
 smt.
 qed.
 
